developFiles/02kleisli_flows/nd_funs/cat2funcset.thy
@@ -1,6 +1,6 @@
-theory cat2rel
-  imports cat2rel_pre
-
+theory cat2funcset
+  imports cat2funcset_pre
+                        
 begin
 
 section{* Hybrid System Verification *}
@@ -42,24 +42,24 @@ lemma (in local_flow) "\<R> (\<lambda> s. orbit s) = {(s, \<phi> t s)|s t. t \<i
   apply(safe, simp_all add: f2r_def)
   by(rule_tac x="t" in exI, simp)
 
-theorem (in local_flow) wp_orbit:"wp (\<R> (\<lambda> s. orbit s)) \<lceil>Q\<rceil> = \<lceil>\<lambda> s. \<forall> t \<in> T. s \<in> S \<longrightarrow> Q (\<phi> t s)\<rceil>"
-  unfolding f2r_def by (subst wp_rel, auto)
+theorem (in local_flow) wp_orbit:"wp (orbit\<^sup>\<bullet>) \<lceil>Q\<rceil> = \<lceil>\<lambda> s. \<forall> t \<in> T. s \<in> S \<longrightarrow> Q (\<phi> t s)\<rceil>"
+  by(subst wp_nd_fun, rule nd_fun_ext, auto)
 
 abbreviation 
-g_orbit :: "(('a::banach) \<Rightarrow> 'a) \<Rightarrow> real set \<Rightarrow> 'a set \<Rightarrow> real \<Rightarrow> 'a pred \<Rightarrow> 'a rel" ("(1{[x\<acute>=_]_ _ @ _ & _})")
-where "{[x\<acute>=f]T S @ t0 & G} \<equiv> \<R> (\<lambda> s. g_orbital (\<lambda> t. f) T S t0 s G)"
+g_orbit ::"(('a::banach)\<Rightarrow>'a) \<Rightarrow> real set \<Rightarrow> 'a set \<Rightarrow> real \<Rightarrow> 'a pred \<Rightarrow> 'a nd_fun" ("(1{[x\<acute>=_]_ _ @ _ & _})")
+where "{[x\<acute>=f]T S @ t0 & G} \<equiv> (\<lambda> s. g_orbital (\<lambda> t. f) T S t0 s G)\<^sup>\<bullet>"
 
 theorem wp_g_orbit:
   assumes "local_flow f S T L \<phi>"
   shows "wp ({[x\<acute>=f]T S @ 0 & G}) \<lceil>Q\<rceil> = \<lceil>\<lambda> s. \<forall> t \<in> T. s \<in> S \<longrightarrow> (\<forall> r \<in> {0--t}.G (\<phi> r s)) \<longrightarrow> Q (\<phi> t s)\<rceil>"
-  unfolding f2r_def apply(subst wp_rel)
-  using assms apply(subst local_flow.g_orbital_is_orbit, simp)
-  by auto
+  apply(subst wp_nd_fun, rule nd_fun_ext)
+  using assms apply(subst local_flow.g_orbital_is_orbit, simp) by auto
 
 text{* This last theorem allows us to compute weakest liberal preconditions for known systems of ODEs: *}
+
 corollary line_DS:
   assumes "0 \<le> t"
-  shows " wp {[x\<acute>=\<lambda>s. c]{0..t} UNIV @ 0 & G} \<lceil>Q\<rceil> = 
+  shows "wp {[x\<acute>=\<lambda>s. c]{0..t} UNIV @ 0 & G} \<lceil>Q\<rceil> = 
     \<lceil>\<lambda> x. \<forall> \<tau> \<in> {0..t}. (\<forall>r\<in>{0--\<tau>}. G (x + r *\<^sub>R c)) \<longrightarrow> Q (x + \<tau> *\<^sub>R c)\<rceil>"
   apply(subst wp_g_orbit[of "\<lambda> s. c" _ _ "1/(t + 1)" "(\<lambda> t x. x + t *\<^sub>R c)"])
   using line_is_local_flow and assms by (blast, simp)
@@ -73,123 +73,130 @@ Then we prove the inference rules which are used in verification proofs.*}
 
 subsubsection{* Differential Weakening *}
 
+thm kcomp_def kcomp_prop le_fun_def
+        
 theorem DW:
   shows "wp ({[x\<acute>=f]T S @ t0 & G}) \<lceil>Q\<rceil> = wp ({[x\<acute>=f]T S @ t0 & G}) \<lceil>\<lambda> s. G s \<longrightarrow> Q s\<rceil>"
-  unfolding rel_antidomain_kleene_algebra.fbox_def rel_ad_def f2r_def
-  apply(simp add: relcomp.simps p2r_def)
-  apply(rule subset_antisym)
-  by fastforce+
+  unfolding fbox_def apply(rule nd_fun_ext) apply transfer apply simp
+proof(subst kcomp_prop)+
+  fix x::'a and T f S t0 G Q 
+  let ?Y = "g_orbital (\<lambda>a. f) T S t0 x G"
+  have *:"\<forall>y \<in> ?Y. G y" by blast
+  {assume "(\<Union>y\<in>?Y . if \<not> Q y then \<eta> y else {}) = {}"
+    then have "\<forall>y\<in>?Y . (if \<not> Q y then \<eta> y else {}) = {}" by blast
+    hence "\<forall>y\<in>?Y . Q y" by (metis (mono_tags, lifting) bot_pres_del) 
+    then have "\<forall>y\<in>?Y . (if G y \<and> \<not> Q y then \<eta> y else {}) = {}" by auto
+    from this have "(\<Union>y\<in>?Y . if G y \<and> \<not> Q y then \<eta> y else {}) = {}" by blast}
+  moreover
+  {assume "(\<Union>y\<in>?Y .  if \<not> Q y then \<eta> y else {}) \<noteq> {}"
+    then have "\<exists>y\<in>?Y. (if \<not> Q y then \<eta> y else {}) \<noteq> {}" by blast
+    hence "\<exists>y\<in>?Y. \<not> Q y" by (metis (mono_tags, lifting)) 
+    then have "\<exists>y\<in>?Y. (if G y \<and> \<not> Q y then \<eta> y else {}) \<noteq> {}"
+      by (metis (mono_tags, lifting) * bot_pres_del) 
+    from this have "(\<Union>y\<in>?Y. if G y \<and> \<not> Q y then \<eta> y else {}) \<noteq> {}" by blast}
+  ultimately show "((\<Union>y\<in>?Y. if \<not> Q y then \<eta> y else {}) = {} \<longrightarrow>
+        (\<Union>y\<in>?Y. if G y \<and> \<not> Q y then \<eta> y else {}) = {}) \<and>
+       ((\<Union>y\<in>?Y. if \<not> Q y then \<eta> y else {}) \<noteq> {} \<longrightarrow>
+        (\<Union>y\<in>?Y. if G y \<and> \<not> Q y then \<eta> y else {}) \<noteq> {})"
+    by blast
+qed
 
 theorem dWeakening: 
-assumes "\<lceil>G\<rceil> \<subseteq> \<lceil>Q\<rceil>"
-shows "\<lceil>P\<rceil> \<subseteq> wp ({[x\<acute>=f]T S @ t0 & G}) \<lceil>Q\<rceil>"
-  using assms apply(subst wp_rel)
-  by(auto simp: f2r_def)
+assumes "\<lceil>G\<rceil> \<le> \<lceil>Q\<rceil>"
+shows "\<lceil>P\<rceil> \<le> wp ({[x\<acute>=f]T S @ t0 & G}) \<lceil>Q\<rceil>"
+  using assms apply(subst wp_nd_fun)
+  by(auto simp: le_fun_def)
 
 subsubsection{* Differential Cut *}
 
-lemma wp_g_orbit_IdD:
-  assumes "wp ({[x\<acute>=f]T S @ t0 & G}) \<lceil>C\<rceil> = Id" and "\<forall> r\<in>{t0--t}. (a, x r) \<in> {[x\<acute>=f]T S @ t0 & G}"
+lemma wp_g_orbit_etaD:
+  assumes "wp ({[x\<acute>=f]T S @ t0 & G}) \<lceil>C\<rceil> = \<eta>\<^sup>\<bullet>" and "\<forall> r\<in>{t0--t}. x r \<in> g_orbital (\<lambda>t. f) T S t0 a G"
   shows "\<forall>r\<in>{t0--t}. C (x r)"
-proof-
-  {fix r :: real
-    have "\<And>R P s. wp R \<lceil>P\<rceil> \<noteq> Id \<or> (\<forall>y. (s::'a, y) \<in> R \<longrightarrow> P y)"
-      by (metis (lifting) p2r_IdD wp_rel)
-    then have "r \<notin> {t0--t} \<or> C (x r)" using assms by blast}
-  then show ?thesis by blast
+proof
+  fix r assume "r \<in> {t0--t}"
+  then have "x r \<in> g_orbital (\<lambda>t. f) T S t0 a G" 
+    using assms(2) by blast
+  also have "\<forall>y. y \<in> (g_orbital (\<lambda>t. f) T S t0 a G) \<longrightarrow> C y" 
+    using assms(1) wp_nd_fun_etaD by fastforce
+  ultimately show "C (x r)" by blast
 qed
 
 theorem DC:
-  assumes "t0 \<in> T" and "interval T"
-    and "wp ({[x\<acute>=f]T S @ t0 & G}) \<lceil>C\<rceil> = Id"
-  shows "wp ({[x\<acute>=f]T S @ t0 & G}) \<lceil>Q\<rceil> = wp {[x\<acute>=f]T S @ t0 & \<lambda>s. G s \<and> C s} \<lceil>Q\<rceil>"
-proof(rule_tac f="\<lambda> x. wp x \<lceil>Q\<rceil>" in HOL.arg_cong, safe)
-  fix a b assume "(a, b) \<in> {[x\<acute>=f]T S @ t0 & G}" 
-  then obtain t::real and x where "t \<in> T" and x_solves:"(x solves_ode (\<lambda>t. f)) T S" and 
+  assumes "picard_ivp (\<lambda> t. f) T S L t0" 
+    and "wp ({[x\<acute>=f]T S @ t0 & G}) \<lceil>C\<rceil> = \<eta>\<^sup>\<bullet>"
+  shows "wp ({[x\<acute>=f]T S @ t0 & G}) \<lceil>Q\<rceil> = wp ({[x\<acute>=f]T S @ t0 & \<lambda>s. G s \<and> C s}) \<lceil>Q\<rceil>"
+proof(rule_tac f="\<lambda> x. wp x \<lceil>Q\<rceil>" in HOL.arg_cong, rule nd_fun_ext, rule subset_antisym, simp_all)
+  fix a
+  show "g_orbital (\<lambda>a. f) T S t0 a G \<subseteq> g_orbital (\<lambda>a. f) T S t0 a (\<lambda>s. G s \<and> C s)"
+  proof
+    fix b assume "b \<in> g_orbital (\<lambda>a. f) T S t0 a G" 
+    then obtain t::real and x where "t \<in> T" and x_solves:"(x solves_ode (\<lambda>t. f)) T S" and 
     "x t0 = a" and guard_x:"(\<forall>r\<in>{t0--t}. G (x r))" and "a \<in> S" and "b = x t"
-    unfolding f2r_def by blast
-  from guard_x have "\<forall>r\<in>{t0--t}.\<forall> \<tau>\<in>{t0--r}. G (x \<tau>)"
-    using assms(1) by (metis contra_subsetD ends_in_segment(1) subset_segment(1)) 
-  also have "\<forall>r\<in>{t0--t}. r \<in> T"
-    using assms(1,2) \<open>t \<in> T\<close> interval.closed_segment_subset_domain by blast
-  ultimately have "\<forall>r\<in>{t0--t}. (a, x r) \<in> {[x\<acute>=f]T S @ t0 & G}"
-    using x_solves \<open>x t0 = a\<close> \<open>a \<in> S\<close> unfolding f2r_def by blast 
-  from this have "\<forall>r\<in>{t0--t}. C (x r)" using wp_g_orbit_IdD assms(3) by blast
-  thus "(a, b) \<in> {[x\<acute>=f]T S @ t0 & \<lambda>s. G s \<and> C s}"
-    using guard_x \<open>a \<in> S\<close> \<open>b = x t\<close> \<open>t \<in> T\<close> \<open>x t0 = a\<close> f2r_def x_solves by fastforce 
-next
-  fix a b assume "(a, b) \<in> {[x\<acute>=f]T S @ t0 & \<lambda>s. G s \<and> C s}" 
-  then show "(a, b) \<in> {[x\<acute>=f]T S @ t0 & G}"
-    unfolding f2r_def by blast
+      using assms(1) unfolding f2r_def by blast
+    from guard_x have "\<forall>r\<in>{t0--t}.\<forall> \<tau>\<in>{t0--r}. G (x \<tau>)"
+      using assms(1) by (metis contra_subsetD ends_in_segment(1) subset_segment(1))
+    also have "\<forall>r\<in>{t0--t}. r \<in> T"
+      using assms(1) \<open>t \<in> T\<close> picard_ivp.subsegment picard_ivp.init_time by blast
+    ultimately have "\<forall> r\<in>{t0--t}. x r \<in> g_orbital (\<lambda>t. f) T S t0 a G"
+      using x_solves \<open>x t0 = a\<close> \<open>a \<in> S\<close> unfolding f2r_def by blast 
+    from this have "\<forall>r\<in>{t0--t}. C (x r)" using wp_g_orbit_etaD assms(2) by blast
+    thus "b \<in> g_orbital (\<lambda>t. f) T S t0 a (\<lambda> s. G s \<and> C s)"
+      using guard_x \<open>a \<in> S\<close> \<open>b = x t\<close> \<open>t \<in> T\<close> \<open>x t0 = a\<close> f2r_def x_solves by fastforce 
+  qed
+next show "\<And> a. g_orbital (\<lambda>t. f) T S t0 a (\<lambda> s. G s \<and> C s) \<subseteq> g_orbital (\<lambda>t. f) T S t0 a G" by auto
 qed
 
 theorem dCut:
   assumes "t0 \<in> T" and "interval T"
-    and wp_C:"\<lceil>P\<rceil> \<subseteq> wp ({[x\<acute>=f]T S @ t0 & G}) \<lceil>C\<rceil>"
-    and wp_Q:"\<lceil>P\<rceil> \<subseteq> wp ({[x\<acute>=f]T S @ t0 & (\<lambda> s. G s \<and> C s)}) \<lceil>Q\<rceil>"
-  shows "\<lceil>P\<rceil> \<subseteq> wp ({[x\<acute>=f]T S @ t0 & G}) \<lceil>Q\<rceil>"
-proof(subst wp_rel, simp add: p2r_def, clarsimp)
-  fix a y assume "P a" and "(a, y) \<in> {[x\<acute>=f]T S @ t0 & G}"
-  then obtain x t where "t \<in> T" and x_solves:"(x solves_ode (\<lambda> t s. f s))T S " and "x t = y"
-    and "x t0 = a" and guard_x:"(\<forall> r \<in> {t0--t}. G (x r))"  and "a \<in> S" by(auto simp: f2r_def)
+    and wp_C:"\<lceil>P\<rceil> \<le> wp ({[x\<acute>=f]T S @ t0 & G}) \<lceil>C\<rceil>"
+    and wp_Q:"\<lceil>P\<rceil> \<le> wp ({[x\<acute>=f]T S @ t0 & (\<lambda> s. G s \<and> C s)}) \<lceil>Q\<rceil>"
+  shows "\<lceil>P\<rceil> \<le> wp ({[x\<acute>=f]T S @ t0 & G}) \<lceil>Q\<rceil>"
+proof(subst wp_nd_fun, clarsimp)
+  fix t::real and x::"real \<Rightarrow> 'a" assume "P (x t0)" and "t \<in> T"  and "x t0 \<in> S"
+and x_solves:"(x solves_ode (\<lambda> t s. f s))T S " and guard_x:"(\<forall> r \<in> {t0--t}. G (x r))"
   from guard_x have "\<forall>r\<in>{t0--t}.\<forall> \<tau>\<in>{t0--r}. G (x \<tau>)"
-    using assms(1) by (metis contra_subsetD ends_in_segment(1) subset_segment(1)) 
+    using \<open>t0 \<in> T\<close> by (metis contra_subsetD ends_in_segment(1) subset_segment(1)) 
   also have "\<forall>r\<in>{t0--t}. r \<in> T"
-    using assms(1,2) \<open>t \<in> T\<close> interval.closed_segment_subset_domain by blast
-  ultimately have "\<forall>r\<in>{t0--t}. (a, x r) \<in> {[x\<acute>=f]T S @ t0 & G}"
-    using x_solves \<open>x t0 = a\<close> \<open>a \<in> S\<close> unfolding f2r_def by blast
-  from this have "\<forall>r\<in>{t0--t}. C (x r)" using assms(3) \<open>P a\<close> by(subst (asm) wp_rel) auto
-  hence "(a, y) \<in> {[x\<acute>=f]T S @ t0 & \<lambda>s. G s \<and> C s}"
-    using guard_x \<open>a \<in> S\<close> \<open>x t = y\<close> \<open>t \<in> T\<close> \<open>x t0 = a\<close> f2r_def x_solves by fastforce 
-  from this \<open>P a\<close> and wp_Q show "Q y"
-    by(subst (asm) wp_rel, simp add: f2r_def)
+    using \<open>t0 \<in> T\<close> \<open>interval T\<close> \<open>t \<in> T\<close> interval.closed_segment_subset_domain by blast
+  ultimately have "\<forall>r\<in>{t0--t}. x r \<in> g_orbital (\<lambda>a. f) T S t0 (x t0) G"
+    using x_solves \<open>x t0 \<in> S\<close> by blast
+  from this have "\<forall>r\<in>{t0--t}. C (x r)" using wp_C \<open>P (x t0)\<close> by(subst (asm) wp_nd_fun, simp)
+  hence "x t \<in> g_orbital (\<lambda>a. f) T S t0 (x t0) (\<lambda> s. G s \<and> C s)"
+    using guard_x  \<open>t \<in> T\<close>  x_solves \<open>x t0 \<in> S\<close> by fastforce
+  from this \<open>P (x t0)\<close> and wp_Q show "Q (x t)"
+    by(subst (asm) wp_nd_fun, simp)
 qed
 
 corollary dCut_interval:
-  assumes "t0 \<le> t" and "\<lceil>P\<rceil> \<subseteq> wp ({[x\<acute>=f]{t0..t} S @ t0 & G}) \<lceil>C\<rceil>" 
-    and "\<lceil>P\<rceil> \<subseteq> wp ({[x\<acute>=f]{t0..t} S @ t0 & (\<lambda> s. G s \<and> C s)}) \<lceil>Q\<rceil>"
-  shows "\<lceil>P\<rceil> \<subseteq> wp ({[x\<acute>=f]{t0..t} S @ t0 & G}) \<lceil>Q\<rceil>"
+  assumes "t0 \<le> t" and "\<lceil>P\<rceil> \<le> wp ({[x\<acute>=f]{t0..t} S @ t0 & G}) \<lceil>C\<rceil>" 
+    and "\<lceil>P\<rceil> \<le> wp ({[x\<acute>=f]{t0..t} S @ t0 & (\<lambda> s. G s \<and> C s)}) \<lceil>Q\<rceil>"
+  shows "\<lceil>P\<rceil> \<le> wp ({[x\<acute>=f]{t0..t} S @ t0 & G}) \<lceil>Q\<rceil>"
   apply(rule_tac C="C" in dCut)
   using assms by(simp_all add: interval_def)
 
 subsubsection{* Differential Invariant *}
 
 lemma DI_sufficiency:
-  assumes picard:"picard_ivp (\<lambda> t. f) T S L t0"
-  shows "wp {[x\<acute>=f]T S @ t0 & G} \<lceil>Q\<rceil> \<subseteq> wp \<lceil>G\<rceil> \<lceil>\<lambda>s. s \<in> S \<longrightarrow> Q s\<rceil>"
-proof(subst wp_rel, subst wp_rel, simp add: p2r_def, clarsimp)
-  fix s assume wlpQ:"\<forall>y. (s, y) \<in> {[x\<acute>=f]T S @ t0 & G} \<longrightarrow> Q y" and "s \<in> S" and "G s"
-  from this and picard obtain x where "(x solves_ode (\<lambda> t. f))T S \<and> x t0 = s"
-    using picard_ivp.fixed_point_solves by blast
-  then also have "\<forall> r \<in> {t0--t0}. G (x r)" using \<open>G s\<close> by simp 
-  ultimately have "(s,s) \<in> {[x\<acute>=f]T S @ t0 & G}"
-    using picard picard_ivp.init_time \<open>s \<in> S\<close> f2r_def by fastforce
-  thus "Q s" using wlpQ by blast
-qed
+  assumes "picard_ivp (\<lambda> t. f) T S L t0"
+  shows "wp {[x\<acute>=f]T S @ t0 & G} \<lceil>Q\<rceil> \<le> wp \<lceil>G\<rceil> \<lceil>\<lambda>s. s \<in> S \<longrightarrow> Q s\<rceil>"
+  apply(subst wp_nd_fun, subst wp_nd_fun, clarsimp)
+  apply(erule_tac x="s" in allE, erule impE, rule_tac x="t0" in exI, simp_all)
+  using assms picard_ivp.fixed_point_solves picard_ivp.init_time by metis
 
 lemma dInvariant:
   fixes \<theta>::"'a::banach \<Rightarrow> real"
-  assumes "\<lceil>G\<rceil> \<subseteq> \<lceil>F\<rceil>" and "bdd_below T"
+  assumes "\<lceil>G\<rceil> \<le> \<lceil>F\<rceil>" and "bdd_below T"
     and FisPrimedI:"\<forall> x. (x solves_ode (\<lambda> t. f))T S \<longrightarrow> I (x (Inf T)) \<longrightarrow>
     (\<forall> t \<in> T. (\<forall>r\<in>{(Inf T)--t}. F (x r)) \<longrightarrow> (I (x t)))"
-  shows "\<lceil>I\<rceil> \<subseteq> wp ({[x\<acute>=f]T S @ (Inf T) & G}) \<lceil>I\<rceil>"
-proof(subst wp_rel, simp add: p2r_def, clarsimp)
-  fix s y assume "(s,y) \<in> {[x\<acute>=f]T S @ (Inf T) & G}" and sHyp:"I s"
-  then obtain x and t where x_ivp:"(x solves_ode (\<lambda> t. f))T S \<and> x (Inf T) = s" 
-    and xtHyp:"x t = y \<and> t \<in> T" and GHyp:"\<forall>r\<in>{(Inf T)--t}. G (x r)" 
-    by(simp add: f2r_def, clarify, auto)
-  hence "(Inf T) \<le> t" by (simp add: \<open>bdd_below T\<close> cInf_lower)
-  from GHyp and \<open>\<lceil>G\<rceil> \<subseteq> \<lceil>F\<rceil>\<close> have geq0:"\<forall>r\<in>{(Inf T)--t}. F (x r)"
-    by (auto simp: p2r_def)
-  thus "I y" using xtHyp x_ivp sHyp and FisPrimedI by blast 
-qed
+  shows "\<lceil>I\<rceil> \<le> wp ({[x\<acute>=f]T S @ (Inf T) & G}) \<lceil>I\<rceil>"
+  using assms apply(subst wp_nd_fun) by clarsimp
 
 lemma invariant_eq_0:
   fixes \<theta>::"'a::banach \<Rightarrow> real"
   assumes nuHyp:"\<forall> x. (x solves_ode (\<lambda> t. f))T S \<longrightarrow> (\<forall> t \<in> T. \<forall> r \<in> {(Inf T)--t}. 
   ((\<lambda>\<tau>. \<theta> (x \<tau>)) has_derivative (\<lambda>\<tau>. \<tau> *\<^sub>R \<nu> (x r))) (at r within {(Inf T)--t}))"
-    and "\<lceil>G\<rceil> \<subseteq> \<lceil>\<lambda>s. \<nu> s = 0\<rceil>" and "bdd_below T"
-  shows "\<lceil>\<lambda>s. \<theta> s = 0\<rceil> \<subseteq> wp ({[x\<acute>=f]T S @ (Inf T) & G}) \<lceil>\<lambda>s. \<theta> s = 0\<rceil>"
+    and "\<lceil>G\<rceil> \<le> \<lceil>\<lambda>s. \<nu> s = 0\<rceil>" and "bdd_below T"
+  shows "\<lceil>\<lambda>s. \<theta> s = 0\<rceil> \<le> wp ({[x\<acute>=f]T S @ (Inf T) & G}) \<lceil>\<lambda>s. \<theta> s = 0\<rceil>"
   apply(rule dInvariant [of _ "\<lambda> s. \<nu> s = 0"])
   using assms apply(simp, simp)
 proof(clarify)
@@ -211,9 +218,9 @@ corollary invariant_eq_0_interval:
   fixes \<theta>::"'a::banach \<Rightarrow> real"
   assumes "\<forall> x. (x solves_ode (\<lambda> t. f)){t0..t} S \<longrightarrow> (\<forall> \<tau> \<in> {t0..t}. \<forall> r \<in> {t0..\<tau>}. 
   ((\<lambda>\<tau>. \<theta> (x \<tau>)) has_derivative (\<lambda>\<tau>. \<tau> *\<^sub>R (\<nu> (x r)))) (at r within {t0..\<tau>}))"
-    and "\<lceil>G\<rceil> \<subseteq> \<lceil>\<lambda>s. \<nu> s = 0\<rceil>" and "t0 \<le> t"
-  shows "\<lceil>\<lambda>s. \<theta> s = 0\<rceil> \<subseteq> wp ({[x\<acute>=f]{t0..t} S @ t0 & G}) \<lceil>\<lambda>s. \<theta> s = 0\<rceil>"
-  apply(subgoal_tac "\<lceil>\<lambda>s. \<theta> s = 0\<rceil> \<subseteq> wp ({[x\<acute>=f]{t0..t} S @ (Inf {t0..t}) & G}) \<lceil>\<lambda>s. \<theta> s = 0\<rceil>")
+    and "\<lceil>G\<rceil> \<le> \<lceil>\<lambda>s. \<nu> s = 0\<rceil>" and "t0 \<le> t"
+  shows "\<lceil>\<lambda>s. \<theta> s = 0\<rceil> \<le> wp ({[x\<acute>=f]{t0..t} S @ t0 & G}) \<lceil>\<lambda>s. \<theta> s = 0\<rceil>"
+  apply(subgoal_tac "\<lceil>\<lambda>s. \<theta> s = 0\<rceil> \<le> wp ({[x\<acute>=f]{t0..t} S @ (Inf {t0..t}) & G}) \<lceil>\<lambda>s. \<theta> s = 0\<rceil>")
    apply(subgoal_tac "Inf {t0..t} = t0", simp)
   using \<open>t0 \<le> t\<close> apply simp
   apply(rule invariant_eq_0[of _ "{t0..t}" _ _ \<nu>])
@@ -223,22 +230,21 @@ theorem dInvariant_eq_0:
   fixes \<theta>::"'a::banach \<Rightarrow> real" and \<nu>::"'a \<Rightarrow> real"
   assumes "\<forall>x. (x solves_ode (\<lambda>t. f)) {t0..t} S \<longrightarrow> 
   (\<forall>\<tau>\<in>{t0..t}. \<forall>r\<in>{t0..\<tau>}. ((\<lambda>\<tau>. \<theta> (x \<tau>)) has_derivative (\<lambda>\<tau>. \<tau> *\<^sub>R \<nu> (x r))) (at r within {t0..\<tau>}))"
-    and impls:"\<lceil>P\<rceil> \<subseteq> \<lceil>\<lambda>s. \<theta> s = 0\<rceil>" "\<lceil>\<lambda>s. \<theta> s = 0\<rceil> \<subseteq> \<lceil>Q\<rceil>" "\<lceil>G\<rceil> \<subseteq> \<lceil>\<lambda>s. \<nu> s = 0\<rceil>" and "t0 \<le> t"
-  shows "\<lceil>P\<rceil> \<subseteq> wp ({[x\<acute>=f]{t0..t} S @ t0 & G}) \<lceil>Q\<rceil>"
+    and impls:"\<lceil>P\<rceil> \<le> \<lceil>\<lambda>s. \<theta> s = 0\<rceil>" "\<lceil>\<lambda>s. \<theta> s = 0\<rceil> \<le> \<lceil>Q\<rceil>" "\<lceil>G\<rceil> \<le> \<lceil>\<lambda>s. \<nu> s = 0\<rceil>" and "t0 \<le> t"
+  shows "\<lceil>P\<rceil> \<le> wp ({[x\<acute>=f]{t0..t} S @ t0 & G}) \<lceil>Q\<rceil>"
   apply(rule_tac C="\<lambda>s. \<theta> s = 0" in dCut_interval, simp add: \<open>t0 \<le> t\<close>)
-   apply(subgoal_tac "\<lceil>\<lambda>s. \<theta> s = 0\<rceil> \<subseteq> wp ({[x\<acute>=f]{t0..t} S @ t0 & G}) \<lceil>\<lambda>s. \<theta> s = 0\<rceil>")
-  using impls apply blast
+   apply(subgoal_tac "\<lceil>\<lambda>s. \<theta> s = 0\<rceil> \<le> wp ({[x\<acute>=f]{t0..t} S @ t0 & G}) \<lceil>\<lambda>s. \<theta> s = 0\<rceil>")
+  using impls apply(subst (asm) wp_nd_fun, subst wp_nd_fun) apply auto[1]
    apply(rule_tac \<nu>="\<nu>" in invariant_eq_0_interval)
   using assms(1,4,5) apply(simp, simp, simp)
-  apply(rule dWeakening)
-  using impls by simp
+  apply(rule dWeakening) using impls by auto
 
 lemma invariant_geq_0:
   fixes \<theta>::"'a::banach \<Rightarrow> real"
   assumes nuHyp:"\<forall> x. (x solves_ode (\<lambda> t. f))T S \<longrightarrow> (\<forall> t \<in> T. \<forall> r \<in> {(Inf T)--t}. 
   ((\<lambda>\<tau>. \<theta> (x \<tau>)) has_derivative (\<lambda>\<tau>. \<tau> *\<^sub>R (\<nu> (x r)))) (at r within {(Inf T)--t}))"
-    and "\<lceil>G\<rceil> \<subseteq> \<lceil>\<lambda>s. (\<nu> s) \<ge> 0\<rceil>" and "bdd_below T"
-  shows "\<lceil>\<lambda>s. \<theta> s \<ge> 0\<rceil> \<subseteq> wp ({[x\<acute>=f]T S @ (Inf T) & G}) \<lceil>\<lambda>s. \<theta> s \<ge> 0\<rceil>"
+    and "\<lceil>G\<rceil> \<le> \<lceil>\<lambda>s. (\<nu> s) \<ge> 0\<rceil>" and "bdd_below T"
+  shows "\<lceil>\<lambda>s. \<theta> s \<ge> 0\<rceil> \<le> wp ({[x\<acute>=f]T S @ (Inf T) & G}) \<lceil>\<lambda>s. \<theta> s \<ge> 0\<rceil>"
   apply(rule dInvariant [of _ "\<lambda> s. \<nu> s \<ge> 0"])
   using assms apply(simp, simp)
 proof(clarify)
@@ -259,9 +265,9 @@ corollary invariant_geq_0_interval:
   fixes \<theta>::"'a::banach \<Rightarrow> real"
   assumes "\<forall> x. (x solves_ode (\<lambda> t. f)){t0..t} S \<longrightarrow> (\<forall> \<tau> \<in> {t0..t}. \<forall> r \<in> {t0..\<tau>}. 
   ((\<lambda>\<tau>. \<theta> (x \<tau>)) has_derivative (\<lambda>\<tau>. \<tau> *\<^sub>R (\<nu> (x r)))) (at r within {t0..\<tau>}))"
-    and "\<lceil>G\<rceil> \<subseteq> \<lceil>\<lambda>s. \<nu> s \<ge> 0\<rceil>" and "t0 \<le> t"
-  shows "\<lceil>\<lambda>s. \<theta> s \<ge> 0\<rceil> \<subseteq> wp ({[x\<acute>=f]{t0..t} S @ t0 & G}) \<lceil>\<lambda>s. \<theta> s \<ge> 0\<rceil>"
-  apply(subgoal_tac "\<lceil>\<lambda>s. \<theta> s \<ge> 0\<rceil> \<subseteq> wp ({[x\<acute>=f]{t0..t} S @ (Inf {t0..t}) & G}) \<lceil>\<lambda>s. \<theta> s \<ge> 0\<rceil>")
+    and "\<lceil>G\<rceil> \<le> \<lceil>\<lambda>s. \<nu> s \<ge> 0\<rceil>" and "t0 \<le> t"
+  shows "\<lceil>\<lambda>s. \<theta> s \<ge> 0\<rceil> \<le> wp ({[x\<acute>=f]{t0..t} S @ t0 & G}) \<lceil>\<lambda>s. \<theta> s \<ge> 0\<rceil>"
+  apply(subgoal_tac "\<lceil>\<lambda>s. \<theta> s \<ge> 0\<rceil> \<le> wp ({[x\<acute>=f]{t0..t} S @ (Inf {t0..t}) & G}) \<lceil>\<lambda>s. \<theta> s \<ge> 0\<rceil>")
    apply(subgoal_tac "Inf {t0..t} = t0", simp)
   using \<open>t0 \<le> t\<close> apply(simp add: closed_segment_eq_real_ivl)
   apply(rule invariant_geq_0[of _ "{t0..t}" _ _ \<nu>])
@@ -271,22 +277,21 @@ theorem dInvariant_geq_0:
   fixes \<theta>::"'a::banach \<Rightarrow> real" and \<nu>::"'a \<Rightarrow> real"
   assumes "\<forall>x. (x solves_ode (\<lambda>t. f)) {t0..t} S \<longrightarrow> 
   (\<forall>\<tau>\<in>{t0..t}. \<forall>r\<in>{t0..\<tau>}. ((\<lambda>\<tau>. \<theta> (x \<tau>)) has_derivative (\<lambda>\<tau>. \<tau> *\<^sub>R \<nu> (x r))) (at r within {t0..\<tau>}))"
-    and impls:"\<lceil>P\<rceil> \<subseteq> \<lceil>\<lambda>s. \<theta> s \<ge> 0\<rceil>" "\<lceil>\<lambda>s. \<theta> s \<ge> 0\<rceil> \<subseteq> \<lceil>Q\<rceil>" "\<lceil>G\<rceil> \<subseteq> \<lceil>\<lambda>s. \<nu> s \<ge> 0\<rceil>" and "t0 \<le> t"
-  shows "\<lceil>P\<rceil> \<subseteq> wp ({[x\<acute>=f]{t0..t} S @ t0 & G}) \<lceil>Q\<rceil>"
+    and impls:"\<lceil>P\<rceil> \<le> \<lceil>\<lambda>s. \<theta> s \<ge> 0\<rceil>" "\<lceil>\<lambda>s. \<theta> s \<ge> 0\<rceil> \<le> \<lceil>Q\<rceil>" "\<lceil>G\<rceil> \<le> \<lceil>\<lambda>s. \<nu> s \<ge> 0\<rceil>" and "t0 \<le> t"
+  shows "\<lceil>P\<rceil> \<le> wp ({[x\<acute>=f]{t0..t} S @ t0 & G}) \<lceil>Q\<rceil>"
   apply(rule_tac C="\<lambda>s. \<theta> s \<ge> 0" in dCut_interval, simp add: \<open>t0 \<le> t\<close>)
-   apply(subgoal_tac "\<lceil>\<lambda>s. \<theta> s \<ge> 0\<rceil> \<subseteq> wp ({[x\<acute>=f]{t0..t} S @ t0 & G}) \<lceil>\<lambda>s. \<theta> s \<ge> 0\<rceil>")
-  using impls apply blast
+   apply(subgoal_tac "\<lceil>\<lambda>s. \<theta> s \<ge> 0\<rceil> \<le> wp ({[x\<acute>=f]{t0..t} S @ t0 & G}) \<lceil>\<lambda>s. \<theta> s \<ge> 0\<rceil>")
+  using impls apply(subst (asm) wp_nd_fun, subst wp_nd_fun) apply auto[1]
   apply(rule_tac \<nu>="\<nu>" in invariant_geq_0_interval)
   using assms(1,4,5) apply(simp, simp, simp)
-  apply(rule dWeakening)
-  using impls by simp
+  apply(rule dWeakening) using impls by auto
 
 lemma invariant_leq_0:
   fixes \<theta>::"'a::banach \<Rightarrow> real"
   assumes nuHyp:"\<forall> x. (x solves_ode (\<lambda> t. f))T S \<longrightarrow> (\<forall> t \<in> T. \<forall> r \<in> {(Inf T)--t}. 
   ((\<lambda>\<tau>. \<theta> (x \<tau>)) has_derivative (\<lambda>\<tau>. \<tau> *\<^sub>R (\<nu> (x r)))) (at r within {(Inf T)--t}))"
-    and "\<lceil>G\<rceil> \<subseteq> \<lceil>\<lambda>s. (\<nu> s) \<le> 0\<rceil>" and "bdd_below T"
-  shows "\<lceil>\<lambda>s. \<theta> s \<le> 0\<rceil> \<subseteq> wp ({[x\<acute>=f]T S @ (Inf T) & G}) \<lceil>\<lambda>s. \<theta> s \<le> 0\<rceil>"
+    and "\<lceil>G\<rceil> \<le> \<lceil>\<lambda>s. (\<nu> s) \<le> 0\<rceil>" and "bdd_below T"
+  shows "\<lceil>\<lambda>s. \<theta> s \<le> 0\<rceil> \<le> wp ({[x\<acute>=f]T S @ (Inf T) & G}) \<lceil>\<lambda>s. \<theta> s \<le> 0\<rceil>"
   apply(rule dInvariant [of _ "\<lambda> s. \<nu> s \<le> 0"])
   using assms apply(simp, simp)
 proof(clarify)
@@ -308,9 +313,9 @@ corollary invariant_leq_0_interval:
   fixes \<theta>::"'a::banach \<Rightarrow> real"
   assumes "\<forall> x. (x solves_ode (\<lambda> t. f)){t0..t} S \<longrightarrow> (\<forall> \<tau> \<in> {t0..t}. \<forall> r \<in> {t0..\<tau>}. 
   ((\<lambda>\<tau>. \<theta> (x \<tau>)) has_derivative (\<lambda>\<tau>. \<tau> *\<^sub>R (\<nu> (x r)))) (at r within {t0..\<tau>}))"
-    and "\<lceil>G\<rceil> \<subseteq> \<lceil>\<lambda>s. \<nu> s \<le> 0\<rceil>" and "t0 \<le> t"
-  shows "\<lceil>\<lambda>s. \<theta> s \<le> 0\<rceil> \<subseteq> wp ({[x\<acute>=f]{t0..t} S @ t0 & G}) \<lceil>\<lambda>s. \<theta> s \<le> 0\<rceil>"
-  apply(subgoal_tac "\<lceil>\<lambda>s. \<theta> s \<le> 0\<rceil> \<subseteq> wp ({[x\<acute>=f]{t0..t} S @ (Inf {t0..t}) & G}) \<lceil>\<lambda>s. \<theta> s \<le> 0\<rceil>")
+    and "\<lceil>G\<rceil> \<le> \<lceil>\<lambda>s. \<nu> s \<le> 0\<rceil>" and "t0 \<le> t"
+  shows "\<lceil>\<lambda>s. \<theta> s \<le> 0\<rceil> \<le> wp ({[x\<acute>=f]{t0..t} S @ t0 & G}) \<lceil>\<lambda>s. \<theta> s \<le> 0\<rceil>"
+  apply(subgoal_tac "\<lceil>\<lambda>s. \<theta> s \<le> 0\<rceil> \<le> wp ({[x\<acute>=f]{t0..t} S @ (Inf {t0..t}) & G}) \<lceil>\<lambda>s. \<theta> s \<le> 0\<rceil>")
    apply(subgoal_tac "Inf {t0..t} = t0", simp)
   using \<open>t0 \<le> t\<close> apply(simp add: closed_segment_eq_real_ivl)
   apply(rule invariant_leq_0[of _ "{t0..t}" _ _ \<nu>])
@@ -320,22 +325,21 @@ theorem dInvariant_leq_0:
   fixes \<theta>::"'a::banach \<Rightarrow> real" and \<nu>::"'a \<Rightarrow> real"
   assumes "\<forall>x. (x solves_ode (\<lambda>t. f)) {t0..t} S \<longrightarrow> 
   (\<forall>\<tau>\<in>{t0..t}. \<forall>r\<in>{t0..\<tau>}. ((\<lambda>\<tau>. \<theta> (x \<tau>)) has_derivative (\<lambda>\<tau>. \<tau> *\<^sub>R \<nu> (x r))) (at r within {t0..\<tau>}))"
-    and impls:"\<lceil>P\<rceil> \<subseteq> \<lceil>\<lambda>s. \<theta> s \<le> 0\<rceil>" "\<lceil>\<lambda>s. \<theta> s \<le> 0\<rceil> \<subseteq> \<lceil>Q\<rceil>" "\<lceil>G\<rceil> \<subseteq> \<lceil>\<lambda>s. \<nu> s \<le> 0\<rceil>" and "t0 \<le> t"
-  shows "\<lceil>P\<rceil> \<subseteq> wp ({[x\<acute>=f]{t0..t} S @ t0 & G}) \<lceil>Q\<rceil>"
+    and impls:"\<lceil>P\<rceil> \<le> \<lceil>\<lambda>s. \<theta> s \<le> 0\<rceil>" "\<lceil>\<lambda>s. \<theta> s \<le> 0\<rceil> \<le> \<lceil>Q\<rceil>" "\<lceil>G\<rceil> \<le> \<lceil>\<lambda>s. \<nu> s \<le> 0\<rceil>" and "t0 \<le> t"
+  shows "\<lceil>P\<rceil> \<le> wp ({[x\<acute>=f]{t0..t} S @ t0 & G}) \<lceil>Q\<rceil>"
   apply(rule_tac C="\<lambda>s. \<theta> s \<le> 0" in dCut_interval, simp add: \<open>t0 \<le> t\<close>)
-   apply(subgoal_tac "\<lceil>\<lambda>s. \<theta> s \<le> 0\<rceil> \<subseteq> wp ({[x\<acute>=f]{t0..t} S @ t0 & G}) \<lceil>\<lambda>s. \<theta> s \<le> 0\<rceil>")
-  using impls apply blast
+   apply(subgoal_tac "\<lceil>\<lambda>s. \<theta> s \<le> 0\<rceil> \<le> wp ({[x\<acute>=f]{t0..t} S @ t0 & G}) \<lceil>\<lambda>s. \<theta> s \<le> 0\<rceil>")
+  using impls apply(subst (asm) wp_nd_fun, subst wp_nd_fun) apply auto[1]
   apply(rule_tac \<nu>="\<nu>" in invariant_leq_0_interval)
   using assms(1,4,5) apply(simp, simp, simp)
-  apply(rule dWeakening)
-  using impls by simp
+  apply(rule dWeakening) using impls by auto
 
 lemma invariant_above_0:
   fixes \<theta>::"'a::banach \<Rightarrow> real"
   assumes nuHyp:"\<forall> x. (x solves_ode (\<lambda> t. f))T S \<longrightarrow>  (\<forall> t \<in> T. \<forall> r \<in> {(Inf T)--t}. 
   ((\<lambda>\<tau>. \<theta> (x \<tau>)) has_derivative (\<lambda>\<tau>. \<tau> *\<^sub>R (\<nu> (x r)))) (at r within {(Inf T)--t}))"
-    and "\<lceil>G\<rceil> \<subseteq> \<lceil>\<lambda>s. (\<nu> s) \<ge> 0\<rceil>" and "bdd_below T"
-  shows "\<lceil>\<lambda>s. \<theta> s > 0\<rceil> \<subseteq> wp ({[x\<acute>=f]T S @ (Inf T) & G}) \<lceil>\<lambda>s. \<theta> s > 0\<rceil>"
+    and "\<lceil>G\<rceil> \<le> \<lceil>\<lambda>s. (\<nu> s) \<ge> 0\<rceil>" and "bdd_below T"
+  shows "\<lceil>\<lambda>s. \<theta> s > 0\<rceil> \<le> wp ({[x\<acute>=f]T S @ (Inf T) & G}) \<lceil>\<lambda>s. \<theta> s > 0\<rceil>"
   apply(rule dInvariant [of _ "\<lambda> s. \<nu> s \<ge> 0"])
   using assms apply(simp, simp)
 proof(clarify)
@@ -358,9 +362,9 @@ corollary invariant_above_0_interval:
   fixes \<theta>::"'a::banach \<Rightarrow> real"
   assumes "\<forall> x. (x solves_ode (\<lambda> t. f)){t0..t} S \<longrightarrow> (\<forall> \<tau> \<in> {t0..t}. \<forall> r \<in> {t0..\<tau>}. 
   ((\<lambda>\<tau>. \<theta> (x \<tau>)) has_derivative (\<lambda>\<tau>. \<tau> *\<^sub>R (\<nu> (x r)))) (at r within {t0..\<tau>}))"
-    and "\<lceil>G\<rceil> \<subseteq> \<lceil>\<lambda>s. \<nu> s \<ge> 0\<rceil>" and "t0 \<le> t"
-  shows "\<lceil>\<lambda>s. \<theta> s > 0\<rceil> \<subseteq> wp ({[x\<acute>=f]{t0..t} S @ t0 & G}) \<lceil>\<lambda>s. \<theta> s > 0\<rceil>"
-  apply(subgoal_tac "\<lceil>\<lambda>s. \<theta> s > 0\<rceil> \<subseteq> wp ({[x\<acute>=f]{t0..t} S @ (Inf {t0..t}) & G}) \<lceil>\<lambda>s. \<theta> s > 0\<rceil>")
+    and "\<lceil>G\<rceil> \<le> \<lceil>\<lambda>s. \<nu> s \<ge> 0\<rceil>" and "t0 \<le> t"
+  shows "\<lceil>\<lambda>s. \<theta> s > 0\<rceil> \<le> wp ({[x\<acute>=f]{t0..t} S @ t0 & G}) \<lceil>\<lambda>s. \<theta> s > 0\<rceil>"
+  apply(subgoal_tac "\<lceil>\<lambda>s. \<theta> s > 0\<rceil> \<le> wp ({[x\<acute>=f]{t0..t} S @ (Inf {t0..t}) & G}) \<lceil>\<lambda>s. \<theta> s > 0\<rceil>")
    apply(subgoal_tac "Inf {t0..t} = t0", simp)
   using \<open>t0 \<le> t\<close> apply(simp add: closed_segment_eq_real_ivl)
   apply(rule invariant_above_0[of _ "{t0..t}" _ _ \<nu>])
@@ -370,22 +374,21 @@ theorem dInvariant_above_0:
   fixes \<theta>::"'a::banach \<Rightarrow> real" and \<nu>::"'a \<Rightarrow> real"
   assumes "\<forall>x. (x solves_ode (\<lambda>t. f)) {t0..t} S \<longrightarrow> 
   (\<forall>\<tau>\<in>{t0..t}. \<forall>r\<in>{t0..\<tau>}. ((\<lambda>\<tau>. \<theta> (x \<tau>)) has_derivative (\<lambda>\<tau>. \<tau> *\<^sub>R \<nu> (x r))) (at r within {t0..\<tau>}))"
-    and impls:"\<lceil>P\<rceil> \<subseteq> \<lceil>\<lambda>s. \<theta> s > 0\<rceil>" "\<lceil>\<lambda>s. \<theta> s > 0\<rceil> \<subseteq> \<lceil>Q\<rceil>" "\<lceil>G\<rceil> \<subseteq> \<lceil>\<lambda>s. \<nu> s \<ge> 0\<rceil>" and "t0 \<le> t"
-  shows "\<lceil>P\<rceil> \<subseteq> wp ({[x\<acute>=f]{t0..t} S @ t0 & G}) \<lceil>Q\<rceil>"
+    and impls:"\<lceil>P\<rceil> \<le> \<lceil>\<lambda>s. \<theta> s > 0\<rceil>" "\<lceil>\<lambda>s. \<theta> s > 0\<rceil> \<le> \<lceil>Q\<rceil>" "\<lceil>G\<rceil> \<le> \<lceil>\<lambda>s. \<nu> s \<ge> 0\<rceil>" and "t0 \<le> t"
+  shows "\<lceil>P\<rceil> \<le> wp ({[x\<acute>=f]{t0..t} S @ t0 & G}) \<lceil>Q\<rceil>"
   apply(rule_tac C="\<lambda>s. \<theta> s > 0" in dCut_interval, simp add: \<open>t0 \<le> t\<close>)
-   apply(subgoal_tac "\<lceil>\<lambda>s. \<theta> s > 0\<rceil> \<subseteq> wp ({[x\<acute>=f]{t0..t} S @ t0 & G}) \<lceil>\<lambda>s. \<theta> s > 0\<rceil>")
-  using impls apply blast
+   apply(subgoal_tac "\<lceil>\<lambda>s. \<theta> s > 0\<rceil> \<le> wp ({[x\<acute>=f]{t0..t} S @ t0 & G}) \<lceil>\<lambda>s. \<theta> s > 0\<rceil>")
+  using impls apply(subst (asm) wp_nd_fun, subst wp_nd_fun) apply auto[1]
   apply(rule_tac \<nu>="\<nu>" in invariant_above_0_interval)
   using assms(1,4,5) apply(simp, simp, simp)
-  apply(rule dWeakening)
-  using impls by simp
+  apply(rule dWeakening) using impls  by auto
 
 lemma invariant_below_0:
   fixes \<theta>::"'a::banach \<Rightarrow> real"
   assumes nuHyp:"\<forall> x. (x solves_ode (\<lambda> t. f))T S \<longrightarrow>  (\<forall> t \<in> T. \<forall> r \<in> {(Inf T)--t}. 
   ((\<lambda>\<tau>. \<theta> (x \<tau>)) has_derivative (\<lambda>\<tau>. \<tau> *\<^sub>R (\<nu> (x r)))) (at r within {(Inf T)--t}))"
-    and "\<lceil>G\<rceil> \<subseteq> \<lceil>\<lambda>s. (\<nu> s) \<le> 0\<rceil>" and "bdd_below T"
-  shows "\<lceil>\<lambda>s. \<theta> s < 0\<rceil> \<subseteq> wp ({[x\<acute>=f]T S @ (Inf T) & G}) \<lceil>\<lambda>s. \<theta> s < 0\<rceil>"
+    and "\<lceil>G\<rceil> \<le> \<lceil>\<lambda>s. (\<nu> s) \<le> 0\<rceil>" and "bdd_below T"
+  shows "\<lceil>\<lambda>s. \<theta> s < 0\<rceil> \<le> wp ({[x\<acute>=f]T S @ (Inf T) & G}) \<lceil>\<lambda>s. \<theta> s < 0\<rceil>"
   apply(rule dInvariant [of _ "\<lambda> s. \<nu> s \<le> 0"])
   using assms apply(simp, simp)
 proof(clarify)
@@ -406,9 +409,9 @@ corollary invariant_below_0_interval:
   fixes \<theta>::"'a::banach \<Rightarrow> real"
   assumes "\<forall> x. (x solves_ode (\<lambda> t. f)){t0..t} S \<longrightarrow> (\<forall> \<tau> \<in> {t0..t}. \<forall> r \<in> {t0..\<tau>}. 
   ((\<lambda>\<tau>. \<theta> (x \<tau>)) has_derivative (\<lambda>\<tau>. \<tau> *\<^sub>R (\<nu> (x r)))) (at r within {t0..\<tau>}))"
-    and "\<lceil>G\<rceil> \<subseteq> \<lceil>\<lambda>s. \<nu> s \<le> 0\<rceil>" and "t0 \<le> t"
-  shows "\<lceil>\<lambda>s. \<theta> s < 0\<rceil> \<subseteq> wp ({[x\<acute>=f]{t0..t} S @ t0 & G}) \<lceil>\<lambda>s. \<theta> s < 0\<rceil>"
-  apply(subgoal_tac "\<lceil>\<lambda>s. \<theta> s < 0\<rceil> \<subseteq> wp ({[x\<acute>=f]{t0..t} S @ (Inf {t0..t}) & G}) \<lceil>\<lambda>s. \<theta> s < 0\<rceil>")
+    and "\<lceil>G\<rceil> \<le> \<lceil>\<lambda>s. \<nu> s \<le> 0\<rceil>" and "t0 \<le> t"
+  shows "\<lceil>\<lambda>s. \<theta> s < 0\<rceil> \<le> wp ({[x\<acute>=f]{t0..t} S @ t0 & G}) \<lceil>\<lambda>s. \<theta> s < 0\<rceil>"
+  apply(subgoal_tac "\<lceil>\<lambda>s. \<theta> s < 0\<rceil> \<le> wp ({[x\<acute>=f]{t0..t} S @ (Inf {t0..t}) & G}) \<lceil>\<lambda>s. \<theta> s < 0\<rceil>")
    apply(subgoal_tac "Inf {t0..t} = t0", simp)
   using \<open>t0 \<le> t\<close> apply(simp add: closed_segment_eq_real_ivl)
   apply(rule invariant_below_0[of _ "{t0..t}" _ _ \<nu>])
@@ -418,54 +421,55 @@ theorem dInvariant_below_0:
   fixes \<theta>::"'a::banach \<Rightarrow> real"
   assumes "\<forall>x. (x solves_ode (\<lambda>t. f)) {t0..t} S \<longrightarrow> 
   (\<forall>\<tau>\<in>{t0..t}. \<forall>r\<in>{t0..\<tau>}. ((\<lambda>\<tau>. \<theta> (x \<tau>)) has_derivative (\<lambda>\<tau>. \<tau> *\<^sub>R \<nu> (x r))) (at r within {t0..\<tau>}))"
-    and impls:"\<lceil>P\<rceil> \<subseteq> \<lceil>\<lambda>s. \<theta> s < 0\<rceil>" "\<lceil>\<lambda>s. \<theta> s < 0\<rceil> \<subseteq> \<lceil>Q\<rceil>" "\<lceil>G\<rceil> \<subseteq> \<lceil>\<lambda>s. \<nu> s \<le> 0\<rceil>" and "t0 \<le> t"
-  shows "\<lceil>P\<rceil> \<subseteq> wp ({[x\<acute>=f]{t0..t} S @ t0 & G}) \<lceil>Q\<rceil>"
+    and impls:"\<lceil>P\<rceil> \<le> \<lceil>\<lambda>s. \<theta> s < 0\<rceil>" "\<lceil>\<lambda>s. \<theta> s < 0\<rceil> \<le> \<lceil>Q\<rceil>" "\<lceil>G\<rceil> \<le> \<lceil>\<lambda>s. \<nu> s \<le> 0\<rceil>" and "t0 \<le> t"
+  shows "\<lceil>P\<rceil> \<le> wp ({[x\<acute>=f]{t0..t} S @ t0 & G}) \<lceil>Q\<rceil>"
   using \<open>t0 \<le> t\<close> apply(rule_tac C="\<lambda>s. \<theta> s < 0" in dCut_interval, simp add: \<open>t0 \<le> t\<close>)
-   apply(subgoal_tac "\<lceil>\<lambda>s. \<theta> s < 0\<rceil> \<subseteq> wp ({[x\<acute>=f]{t0..t} S @ t0 & G}) \<lceil>\<lambda>s. \<theta> s < 0\<rceil>")
-  using impls apply blast
+   apply(subgoal_tac "\<lceil>\<lambda>s. \<theta> s < 0\<rceil> \<le> wp ({[x\<acute>=f]{t0..t} S @ t0 & G}) \<lceil>\<lambda>s. \<theta> s < 0\<rceil>")
+  using impls apply(subst (asm) wp_nd_fun, subst wp_nd_fun) apply auto[1]
   apply(rule_tac \<nu>="\<nu>" in invariant_below_0_interval)
   using assms(1,4,5) apply(simp, simp, simp)
-  apply(rule dWeakening)
-  using impls by simp
+  apply(rule dWeakening) using impls by auto
 
 lemma invariant_meet:
-  assumes "\<lceil>I1\<rceil> \<subseteq> wp ({[x\<acute>=f]T S @ t0 & G}) \<lceil>I1\<rceil>"
-    and "\<lceil>I2\<rceil> \<subseteq> wp ({[x\<acute>=f]T S @ t0 & G}) \<lceil>I2\<rceil>"
-  shows "\<lceil>\<lambda>s. I1 s \<and> I2 s\<rceil> \<subseteq> wp ({[x\<acute>=f]T S @ t0 & G}) \<lceil>\<lambda>s. I1 s \<and> I2 s\<rceil>"
-  using assms apply(subst (asm) wp_rel, subst (asm) wp_rel)
-  apply(subst wp_rel, simp add: p2r_def)
-  by blast
+  assumes "\<lceil>I1\<rceil> \<le> wp ({[x\<acute>=f]T S @ t0 & G}) \<lceil>I1\<rceil>"
+    and "\<lceil>I2\<rceil> \<le> wp ({[x\<acute>=f]T S @ t0 & G}) \<lceil>I2\<rceil>"
+  shows "\<lceil>\<lambda>s. I1 s \<and> I2 s\<rceil> \<le> wp ({[x\<acute>=f]T S @ t0 & G}) \<lceil>\<lambda>s. I1 s \<and> I2 s\<rceil>"
+  using assms by(subst (asm) wp_nd_fun, subst (asm) wp_nd_fun, subst wp_nd_fun, simp, blast)
 
 theorem dInvariant_meet:
-  assumes "\<lceil>I1\<rceil> \<subseteq> wp ({[x\<acute>=f]{t0..t} S @ t0 & G}) \<lceil>I1\<rceil>" and "\<lceil>I2\<rceil> \<subseteq> wp ({[x\<acute>=f]{t0..t} S @ t0 & G}) \<lceil>I2\<rceil>"
-    and impls:"\<lceil>P\<rceil> \<subseteq> \<lceil>\<lambda>s. I1 s \<and> I2 s\<rceil>" "\<lceil>\<lambda>s. I1 s \<and> I2 s\<rceil> \<subseteq> \<lceil>Q\<rceil>" and "t0 \<le> t"
-  shows "\<lceil>P\<rceil> \<subseteq> wp ({[x\<acute>=f]{t0..t} S @ t0 & G}) \<lceil>Q\<rceil>"
+  assumes "\<lceil>I1\<rceil> \<le> wp ({[x\<acute>=f]{t0..t} S @ t0 & G}) \<lceil>I1\<rceil>" and "\<lceil>I2\<rceil> \<le> wp ({[x\<acute>=f]{t0..t} S @ t0 & G}) \<lceil>I2\<rceil>"
+    and impls:"\<lceil>P\<rceil> \<le> \<lceil>\<lambda>s. I1 s \<and> I2 s\<rceil>" "\<lceil>\<lambda>s. I1 s \<and> I2 s\<rceil> \<le> \<lceil>Q\<rceil>" and "t0 \<le> t"
+  shows "\<lceil>P\<rceil> \<le> wp ({[x\<acute>=f]{t0..t} S @ t0 & G}) \<lceil>Q\<rceil>"
   apply(rule_tac C="\<lambda>s. I1 s \<and> I2 s" in dCut_interval, simp add: \<open>t0 \<le> t\<close>)
-   apply(subgoal_tac "\<lceil>\<lambda>s. I1 s \<and> I2 s\<rceil> \<subseteq> wp ({[x\<acute>=f]{t0..t} S @ t0 & G}) \<lceil>\<lambda>s. I1 s \<and> I2 s\<rceil>")
-  using impls apply blast
+   apply(subgoal_tac "\<lceil>\<lambda>s. I1 s \<and> I2 s\<rceil> \<le> wp ({[x\<acute>=f]{t0..t} S @ t0 & G}) \<lceil>\<lambda>s. I1 s \<and> I2 s\<rceil>")
+  using impls apply(transfer, simp add: le_fun_def) apply auto[1]
     apply(rule invariant_meet)
   using assms(1,2,5) apply(simp, simp)
   apply(rule dWeakening)
   using impls by simp
 
 lemma invariant_join:
-  assumes "\<lceil>I1\<rceil> \<subseteq> wp ({[x\<acute>=f]T S @ t0 & G}) \<lceil>I1\<rceil>"
-    and "\<lceil>I2\<rceil> \<subseteq> wp ({[x\<acute>=f]T S @ t0 & G}) \<lceil>I2\<rceil>"
-  shows "\<lceil>\<lambda>s. I1 s \<or> I2 s\<rceil> \<subseteq> wp ({[x\<acute>=f]T S @ t0 & G}) \<lceil>\<lambda>s. I1 s \<or> I2 s\<rceil>"
-  using assms apply(subst (asm) wp_rel, subst (asm) wp_rel)
-  apply(subst wp_rel, simp add: p2r_def)
-  by blast
+  assumes "\<lceil>I1\<rceil> \<le> wp ({[x\<acute>=f]T S @ t0 & G}) \<lceil>I1\<rceil>"
+    and "\<lceil>I2\<rceil> \<le> wp ({[x\<acute>=f]T S @ t0 & G}) \<lceil>I2\<rceil>"
+  shows "\<lceil>\<lambda>s. I1 s \<or> I2 s\<rceil> \<le> wp ({[x\<acute>=f]T S @ t0 & G}) \<lceil>\<lambda>s. I1 s \<or> I2 s\<rceil>"
+  using assms by(subst (asm) wp_nd_fun, subst (asm) wp_nd_fun, subst wp_nd_fun, simp)
 
 theorem dInvariant_join:
-  assumes "\<lceil>I1\<rceil> \<subseteq> wp ({[x\<acute>=f]{t0..t} S @ t0 & G}) \<lceil>I1\<rceil>" and "\<lceil>I2\<rceil> \<subseteq> wp ({[x\<acute>=f]{t0..t} S @ t0 & G}) \<lceil>I2\<rceil>"
-    and impls:"\<lceil>P\<rceil> \<subseteq> \<lceil>\<lambda>s. I1 s \<or> I2 s\<rceil>" "\<lceil>\<lambda>s. I1 s \<or> I2 s\<rceil> \<subseteq> \<lceil>Q\<rceil>" and "t0 \<le> t"
-  shows "\<lceil>P\<rceil> \<subseteq> wp ({[x\<acute>=f]{t0..t} S @ t0 & G}) \<lceil>Q\<rceil>"
+  assumes "\<lceil>I1\<rceil> \<le> wp ({[x\<acute>=f]{t0..t} S @ t0 & G}) \<lceil>I1\<rceil>" and "\<lceil>I2\<rceil> \<le> wp ({[x\<acute>=f]{t0..t} S @ t0 & G}) \<lceil>I2\<rceil>"
+    and impls:"\<lceil>P\<rceil> \<le> \<lceil>\<lambda>s. I1 s \<or> I2 s\<rceil>" "\<lceil>\<lambda>s. I1 s \<or> I2 s\<rceil> \<le> \<lceil>Q\<rceil>" and "t0 \<le> t"
+  shows "\<lceil>P\<rceil> \<le> wp ({[x\<acute>=f]{t0..t} S @ t0 & G}) \<lceil>Q\<rceil>"
   apply(rule_tac C="\<lambda>s. I1 s \<or> I2 s" in dCut_interval, simp add: \<open>t0 \<le> t\<close>)
-   apply(subgoal_tac "\<lceil>\<lambda>s. I1 s \<or> I2 s\<rceil> \<subseteq> wp ({[x\<acute>=f]{t0..t} S @ t0 & G}) \<lceil>\<lambda>s. I1 s \<or> I2 s\<rceil>")
-  using impls apply blast
+   apply(subgoal_tac "\<lceil>\<lambda>s. I1 s \<or> I2 s\<rceil> \<le> wp ({[x\<acute>=f]{t0..t} S @ t0 & G}) \<lceil>\<lambda>s. I1 s \<or> I2 s\<rceil>")
+  using impls apply(transfer, simp add: le_fun_def) apply auto[1]
     apply(rule invariant_join)
   using assms(1,2,5) apply(simp, simp)
   apply(rule dWeakening)
   using impls by auto
+
+
+locale_deps
+
+thm Rep_nd_fun  Rep_nd_fun_inject Rep_nd_fun_cases Rep_nd_fun_inverse
+thm           Abs_nd_fun_inject Abs_nd_fun_cases Abs_nd_fun_inverse 
 
 end
